CC: Add a new type constructor `cpoly`

Semantic/CC/Syntax/Ty.lean
@@ -15,23 +15,44 @@ inductive TySort : Type where
 -- Existential types
 | exi : TySort
 
+inductive CaptureBound : Sig -> Type where
+| unbound : CaptureBound s
+| bound : CaptureSet s -> CaptureBound s
+
 inductive Ty : TySort -> Sig -> Type where
 -- shape types
 | top : Ty .shape s
 | tvar : BVar s .tvar -> Ty .shape s
 | arrow : Ty .capt s -> Ty .exi (s,x) -> Ty .shape s
-| poly : Ty .shape s -> Ty .shape (s,X) -> Ty .shape s
+| poly : Ty .shape s -> Ty .exi (s,X) -> Ty .shape s
+| cpoly : CaptureBound s -> Ty .exi (s,C) -> Ty .shape s
 -- capturing types
 | capt : CaptureSet s -> Ty .shape s -> Ty .capt s
 -- existential types
 | exi : Ty .capt (s,C) -> Ty .exi s
 | typ : Ty .capt s -> Ty .exi s
 
+def CaptureBound.rename : CaptureBound s1 -> Rename s1 s2 -> CaptureBound s2
+| .unbound, _ => .unbound
+| .bound cs, f => .bound (cs.rename f)
+
+def CaptureBound.rename_id {cb : CaptureBound s} : cb.rename (Rename.id) = cb := by
+  cases cb
+  case unbound => rfl
+  case bound cs => simp [CaptureBound.rename, CaptureSet.rename_id]
+
+theorem CaptureBound.rename_comp {cb : CaptureBound s1} {f : Rename s1 s2} {g : Rename s2 s3} :
+    (cb.rename f).rename g = cb.rename (f.comp g) := by
+  cases cb
+  case unbound => rfl
+  case bound cs => simp [CaptureBound.rename, CaptureSet.rename_comp]
+
 def Ty.rename : Ty sort s1 -> Rename s1 s2 -> Ty sort s2
 | .top, _ => .top
 | .tvar x, f => .tvar (f.var x)
 | .arrow T1 T2, f => .arrow (T1.rename f) (T2.rename (f.lift))
 | .poly T1 T2, f => .poly (T1.rename f) (T2.rename (f.lift))
+| .cpoly cb T, f => .cpoly (cb.rename f) (T.rename (f.lift))
 | .capt cs T, f => .capt (cs.rename f) (T.rename f)
 | .exi T, f => .exi (T.rename (f.lift))
 | .typ T, f => .typ (T.rename f)
@@ -42,6 +63,7 @@ def Ty.rename_id {T : Ty sort s} : T.rename (Rename.id) = T := by
   case tvar => rfl
   case arrow ih1 ih2 => simp [Ty.rename, Rename.lift_id, ih1, ih2]
   case poly ih1 ih2 => simp [Ty.rename, Rename.lift_id, ih1, ih2]
+  case cpoly cb ih => simp [Ty.rename, Rename.lift_id, ih, CaptureBound.rename_id]
   case capt ih2 =>
     simp [Ty.rename, ih2, CaptureSet.rename_id]
   case exi ih => simp [Ty.rename, Rename.lift_id, ih]
@@ -54,6 +76,7 @@ theorem Ty.rename_comp {T : Ty sort s1} {f : Rename s1 s2} {g : Rename s2 s3} :
   case tvar => rfl
   case arrow ih1 ih2 => simp [Ty.rename, Rename.lift_comp, ih1, ih2]
   case poly ih1 ih2 => simp [Ty.rename, Rename.lift_comp, ih1, ih2]
+  case cpoly cb ih => simp [Ty.rename, Rename.lift_comp, ih, CaptureBound.rename_comp]
   case capt ih => simp [Ty.rename, CaptureSet.rename_comp, ih]
   case exi ih => simp [Ty.rename, Rename.lift_comp, ih]
   case typ ih => simp [Ty.rename, ih]
